DistinctVars.thy
@@ -1,0 +1,201 @@
+theory DistinctVars
+imports "Nominal-Utils" "~~/src/HOL/Library/AList"
+begin
+
+abbreviation delete where "delete \<equiv> AList.delete"
+
+definition heapVars
+  where "heapVars h = fst ` set h"
+
+lemma heapVarsAppend[simp]:"heapVars (a @ b) = heapVars a \<union> heapVars b"
+  and [simp]:"heapVars ((v,e) # h) = insert v (heapVars h)"
+  and [simp]:"heapVars (p # h) = insert (fst p) (heapVars h)"
+  and [simp]:"heapVars [] = {}"
+  by (auto simp add: heapVars_def)
+
+lemma heapVars_from_set:
+  "(x, e) \<in> set h \<Longrightarrow> x \<in> heapVars h"
+by (induct h, auto)
+
+lemma heapVars_not_fresh:
+  "x \<in> heapVars \<Gamma> \<Longrightarrow> \<not>(atom x \<sharp> \<Gamma>)"
+  by (induct \<Gamma>, auto simp add: fresh_Cons fresh_Pair)
+
+lemma finite_heapVars[simp]:
+  "finite (heapVars \<Gamma>)"
+  by (auto simp add: heapVars_def)
+
+lemma fresh_delete:
+  assumes "atom x \<sharp> \<Gamma>"
+  shows "atom x \<sharp> (delete v \<Gamma>)"
+using assms
+by(induct \<Gamma>)(auto simp add: fresh_Cons)
+
+lemma fresh_heap_expr:
+  assumes "a \<sharp> \<Gamma>"
+  and "(x,e) \<in> set \<Gamma>"
+  shows "a \<sharp> e"
+  using assms
+  by (metis fresh_list_elem fresh_Pair)
+
+lemma fresh_heap_expr':
+  assumes "a \<sharp> \<Gamma>"
+  and "e \<in> snd` set \<Gamma>"
+  shows "a \<sharp> e"
+  using assms
+  by (induct \<Gamma>, auto simp add: fresh_Cons)
+
+lemma fresh_star_heap_expr:
+  assumes "S \<sharp>* \<Gamma>"
+  and "(x,e) \<in> set \<Gamma>"
+  shows "S \<sharp>* e"
+  using assms
+  by (metis fresh_star_def fresh_heap_expr)
+
+lemma fresh_star_heap_expr':
+  assumes "S \<sharp>* \<Gamma>"
+  and "e \<in> snd ` set \<Gamma>"
+  shows "S \<sharp>* e"
+  using assms
+  by (metis fresh_star_def fresh_heap_expr')
+
+
+inductive distinctVars  where
+  [simp]: "distinctVars []" |
+  [intro]:"x \<notin> heapVars \<Gamma> \<Longrightarrow> distinctVars \<Gamma> \<Longrightarrow> distinctVars ((x, e)  # \<Gamma>)"
+
+lemma [simp]: "distinctVars [x]"
+  by (cases x, auto)
+
+lemma heapVars[eqvt]:
+  "\<pi> \<bullet> heapVars \<Gamma> = heapVars (\<pi> \<bullet> \<Gamma>)"
+  apply (simp add: heapVars_def)
+  apply perm_simp
+  apply rule
+  done
+
+lemma distinctVars_eqvt[eqvt]:
+  "distinctVars \<Gamma> \<Longrightarrow> distinctVars (\<pi> \<bullet> \<Gamma>)"
+  apply (induct \<Gamma> rule:distinctVars.induct)
+  apply (auto simp add: heapVars[symmetric] mem_permute_iff)
+  done
+
+lemma distinctVars_appendI:
+  "distinctVars \<Gamma> \<Longrightarrow> distinctVars \<Delta> \<Longrightarrow> heapVars \<Gamma> \<inter> heapVars \<Delta> = {} \<Longrightarrow> distinctVars (\<Gamma> @ \<Delta>)"
+  by (induct \<Gamma> rule:distinctVars.induct, auto)
+
+
+lemma distinctVars_ConsD:
+  assumes "distinctVars ((x,e) # \<Gamma>)"
+  shows "x \<notin> heapVars \<Gamma>" and "distinctVars \<Gamma>"
+  by (rule distinctVars.cases[OF assms], simp_all)+
+
+lemma distinctVars_appendD:
+  assumes "distinctVars (\<Gamma> @ \<Delta>)"
+  shows distinctVars_appendD1: "distinctVars \<Gamma>"
+  and distinctVars_appendD2: "distinctVars \<Delta>"
+  and distinctVars_appendD3: "heapVars \<Gamma> \<inter> heapVars \<Delta> = {}"
+proof-
+  from assms
+  have "distinctVars \<Gamma> \<and> distinctVars \<Delta> \<and> heapVars \<Gamma> \<inter> heapVars \<Delta> = {}"
+  proof (induct \<Gamma> )
+  case Nil thus ?case by simp
+  next
+  case (Cons p \<Gamma>)
+    obtain x e where "p = (x,e)" by (metis PairE)
+    with Cons have "distinctVars ((x,e) # (\<Gamma>@ \<Delta>))" by simp
+    hence "x \<notin> heapVars (\<Gamma>@ \<Delta>)" and "distinctVars (\<Gamma> @ \<Delta>)" by (rule distinctVars_ConsD)+
+
+    from `x \<notin> heapVars (\<Gamma>@ \<Delta>)` have  "x \<notin> heapVars \<Gamma>"  and "x \<notin> heapVars \<Delta>" by auto
+
+    from Cons(1)[OF `distinctVars (\<Gamma> @ \<Delta>)`]
+    have "distinctVars \<Gamma>" and "distinctVars \<Delta>" and "heapVars \<Gamma> \<inter> heapVars \<Delta> = {}" by auto
+    have "distinctVars (p # \<Gamma>)"
+      using `p = _` `x \<notin> heapVars \<Gamma>` `distinctVars \<Gamma>` by auto
+    moreover
+    have "heapVars (p # \<Gamma>) \<inter> heapVars \<Delta> = {}" 
+      using `p = _` `x \<notin> heapVars \<Delta>` `heapVars \<Gamma> \<inter> heapVars \<Delta> = {}` by auto
+    ultimately
+    show ?case using `distinctVars \<Delta>` by auto
+  qed
+  thus "distinctVars \<Gamma>" and "distinctVars \<Delta>" and "heapVars \<Gamma> \<inter> heapVars \<Delta> = {}" by auto
+qed
+
+lemma distinctVars_Cons:
+  "distinctVars (x # \<Gamma>) \<longleftrightarrow> (fst x \<notin> heapVars \<Gamma> \<and> distinctVars \<Gamma>)"
+  by (metis PairE distinctVars.intros(2) distinctVars_ConsD fst_conv)
+
+lemma distinctVars_append:
+  "distinctVars (\<Gamma> @ \<Delta>) \<longleftrightarrow> (distinctVars \<Gamma> \<and> distinctVars \<Delta> \<and> heapVars \<Gamma> \<inter> heapVars \<Delta> = {})"
+  by (metis distinctVars_appendD distinctVars_appendI)
+
+lemma distinctVars_Cons_subset:
+  assumes "heapVars ((x,e)#\<Gamma>) \<subseteq> heapVars ((x,e')#\<Delta>)"
+  assumes "distinctVars ((x,e)#\<Gamma>)"
+  assumes "distinctVars ((x,e')#\<Delta>)"
+  shows "heapVars \<Gamma> \<subseteq> heapVars \<Delta>"
+proof-
+  have "x \<notin> heapVars \<Gamma>" and "x \<notin> heapVars \<Delta>"
+    using assms(2,3) by (metis distinctVars_ConsD(1))+
+  thus ?thesis using assms(1)
+    by auto
+qed
+
+
+lemma delete_no_there:
+  "x \<notin> heapVars \<Gamma> \<Longrightarrow> delete x \<Gamma> = \<Gamma>"
+  by (induct \<Gamma>, auto)
+
+lemma heapVars_delete_subset:
+  "heapVars (delete x \<Gamma>) \<subseteq> heapVars \<Gamma>"
+  by (induct \<Gamma>, auto)
+
+lemma heapVars_delete[simp]:
+  "heapVars (delete x \<Gamma>) = heapVars \<Gamma> - {x}"
+  by (induct \<Gamma>, auto)
+
+lemmas fst_set_delete[simp] = heapVars_delete[unfolded heapVars_def]
+
+lemma distinctVars_delete:
+  "distinctVars \<Gamma> \<Longrightarrow> distinctVars (delete x \<Gamma>)"
+  apply (induct \<Gamma> rule:distinctVars.induct)
+  apply (auto simp add: distinctVars_Cons)
+  done
+
+lemma fresh_heapVars_distinct:
+ assumes "atom ` heapVars \<Delta> \<sharp>* \<Gamma>"
+ shows "heapVars \<Delta> \<inter> heapVars \<Gamma> = {}"
+proof-
+  { fix x
+    assume "x \<in> heapVars \<Delta>"
+    moreover
+    assume "x \<in> heapVars \<Gamma>"
+    hence "atom x \<in> supp \<Gamma>"
+      apply (induct \<Gamma>)
+      by (auto simp add: supp_Cons heapVars_def supp_Pair supp_at_base)
+    ultimately
+    have False
+      using assms
+      by (simp add: fresh_star_def fresh_def)
+  }
+  thus "heapVars \<Delta> \<inter> heapVars \<Gamma> = {}" by auto
+qed
+
+lemma the_map_of_snd:
+  "x\<in> fst ` set \<Gamma> \<Longrightarrow> the (map_of \<Gamma> x) \<in> snd ` set \<Gamma>"
+by (induct \<Gamma>, auto)
+
+lemma distinctVars_set_delete_insert:
+  assumes "distinctVars \<Gamma>"
+  assumes "(x,e) \<in> set \<Gamma>"
+  shows "set ((x,e) # delete x \<Gamma>) = set \<Gamma>"
+  using assms
+  apply (induct \<Gamma> rule:distinctVars.induct)
+  apply auto[1]
+  apply (case_tac "xa = x")
+  apply (auto simp add: heapVars_def)[1]
+    apply (metis fst_conv imageI)
+  apply auto
+  done
+
+end
