HeapToEnv.thy
@@ -1,9 +1,8 @@
 theory "HeapToEnv"
-  imports "Nominal-Utils" "FMap-Nominal-HOLCF"
+  imports "DistinctVars" "Nominal-Utils" "FMap-Nominal-HOLCF"
 begin
 
 default_sort type
-
 
 function heapToEnv :: "('var \<times> 'exp) list \<Rightarrow> ('exp \<Rightarrow> 'value) \<Rightarrow> ('var, 'value) fmap"
 where
@@ -73,5 +72,119 @@ lemma lookupHeapToEnvNotAppend[simp]:
   assumes "x \<notin> fst ` set \<Gamma>"
   shows "the (lookup (heapToEnv (\<Gamma>@h) f) x) = the (lookup (heapToEnv h f) x)"
   using assms by (induct \<Gamma>, auto)
+
+
+lemma heapToEnv_remove_Cons_fmap_expand:
+  "finite S \<Longrightarrow> x \<notin> S \<Longrightarrow> fmap_expand (heapToEnv ((x, e) # \<Gamma>) eval) S = fmap_expand (heapToEnv \<Gamma> eval) S"
+  apply (rule fmap_eqI)
+  apply simp
+  apply (subgoal_tac "xa \<noteq> x")
+  apply (case_tac "xa \<in> fst`set \<Gamma>")
+  apply simp
+  apply simp
+  apply auto
+  done
+
+lemma heapToEnv_mono:
+  "finite d1 \<Longrightarrow>
+   d1 = d2 \<Longrightarrow>
+   x \<notin> fst ` set \<Gamma> \<Longrightarrow>
+  fmap_expand (heapToEnv \<Gamma> eval) d1 \<sqsubseteq> fmap_expand (heapToEnv ((x,e) # \<Gamma>) eval) d2"
+   apply (erule subst)
+   apply (rule fmap_expand_belowI)
+   apply simp
+   apply (rule eq_imp_below)
+   apply simp
+   apply (metis the_lookup_fmap_upd_other[symmetric])
+   done
+
+lemma heapToEnv_reorder_head:
+  assumes "x \<noteq> y"
+  shows "heapToEnv ((x,e1)#(y,e2)#\<Gamma>) eval = heapToEnv ((y,e2)#(x,e1)#\<Gamma>) eval"
+  by (simp add: fmap_upd_twist[OF assms])
+
+lemma heapToEnv_reorder_head_append:
+  assumes "x \<notin> heapVars \<Gamma>"
+  shows "heapToEnv ((x,e)#\<Gamma>@\<Delta>) eval = heapToEnv (\<Gamma> @ ((x,e)#\<Delta>)) eval"
+  using assms
+  apply (induct \<Gamma>)
+  apply simp
+  apply (case_tac a)
+  apply (auto simp del: heapToEnv.simps simp add: heapToEnv_reorder_head)
+  apply simp
+  done
+
+
+
+lemma heapToEnv_delete_insert:
+  assumes "distinctVars \<Gamma>"
+  assumes "(x,e) \<in> set \<Gamma>"
+  shows "heapToEnv \<Gamma> eval = heapToEnv ((x,e) # delete x \<Gamma>) eval"
+using assms
+proof (induct \<Gamma> rule:distinctVars.induct)
+  case goal1 thus ?case by simp
+next
+  case (goal2 y \<Gamma> e2)
+  show ?case
+  proof(cases "(x,e) = (y,e2)")
+  case True
+    from `y \<notin> heapVars \<Gamma>`
+    have "x \<notin> heapVars \<Gamma>" using True by simp
+    hence "delete x \<Gamma> = \<Gamma>" by (rule delete_no_there)
+    with True show ?thesis by simp
+  next
+  case False
+    hence "x \<noteq> y" by (metis goal2(1) goal2(4) heapVars_from_set set_ConsD)
+    hence "(x, e) \<in> set \<Gamma>" by (metis False goal2(4) set_ConsD)
+    note hyp = goal2(3)[OF this]
+
+    have "heapToEnv ((x, e) # delete x ((y, e2) # \<Gamma>)) eval 
+      = heapToEnv ((x, e) # ((y, e2) # delete x \<Gamma>)) eval"
+      using False by simp
+    also have "... = heapToEnv ((y, e2) # ((x, e) # delete x \<Gamma>)) eval"
+      by (rule heapToEnv_reorder_head[OF `x \<noteq> y`])
+    also have "... = heapToEnv ((y, e2) # \<Gamma>) eval"
+      using hyp
+      by simp
+    finally
+    show ?thesis by (rule sym)
+  qed
+qed
+
+lemma heapToEnv_reorder:
+  assumes "distinctVars \<Gamma>"
+  assumes "distinctVars \<Delta>"
+  assumes "set \<Gamma> = set \<Delta>"
+  shows "heapToEnv \<Gamma> eval = heapToEnv \<Delta> eval"
+using assms
+proof (induct \<Gamma> arbitrary: \<Delta> rule:distinctVars.induct)
+case goal1 thus ?case by simp
+next
+case (goal2 x \<Gamma> e \<Delta>)
+  hence "(x,e) \<in> set \<Delta>"
+    by (metis ListMem_iff elem)
+  note Delta' = heapToEnv_delete_insert[OF `distinctVars \<Delta>` this]
+  thm Delta'
+
+  have "distinctVars (delete x \<Delta>)" 
+    by (rule distinctVars_delete[OF goal2(4)])
+  moreover
+  from `set ((x, e) # \<Gamma>) = set \<Delta>`
+  have "set (delete x ((x, e) # \<Gamma>)) = set (delete x \<Delta>)"
+    by (metis project_set delete_eq)
+  hence "set \<Gamma> = set (delete x \<Delta>)"
+    by (simp add: delete_no_there[OF `x \<notin> heapVars \<Gamma>`])
+  ultimately
+  have "heapToEnv \<Gamma> eval = heapToEnv (delete x \<Delta>) eval"
+    by (rule goal2(3))
+  thus ?case
+    by (simp add: Delta')
+qed
+
+lemma heapToEnv_subst_exp:
+  assumes "eval e = eval e'"
+  shows "heapToEnv ((x,e)#\<Gamma>) eval = heapToEnv ((x,e')#\<Gamma>) eval"
+  by (simp add: assms)
+
 
 end
